Don't inline var nodes on the first pass through partial evaluation

src/Experiments/SimplyTypedArithmetic.v
@@ -4263,7 +4263,8 @@ Module Compilers.
 
     Module ident.
       Section interp.
-        Context {var : type -> Type}.
+        Context (inline_var_nodes : bool)
+                {var : type -> Type}.
         Fixpoint is_var_like {t} (e : @expr var t) : bool
           := match e with
              | Var t v => true
@@ -4309,15 +4310,18 @@ Module Compilers.
                              => @interp_let_in
                                   _ B b
                                   (fun b => f (inr (a, b))))
-                     | inl (data, e) => partial.expr.reflect
-                                          (expr_let y := partial.expr.reify (t:=t) x in
-                                               partial.expr.reify (f (inl (data, Var y)%core)))%expr
+                     | inl (data, e)
+                       => if inline_var_nodes && is_var_like e
+                          then f x
+                          else partial.expr.reflect
+                                 (expr_let y := partial.expr.reify (t:=t) x in
+                                      partial.expr.reify (f (inl (data, Var y)%core)))%expr
                      end
              | type.type_primitive _ as t
                => fun (x : data t * expr t + type.interp t) (f : data t * expr t + type.interp t -> value var tC)
                   => match x with
                      | inl (data, e)
-                       => if is_var_like e
+                       => if inline_var_nodes && is_var_like e
                           then f x
                           else partial.expr.reflect
                                  (expr_let y := (partial.expr.reify (t:=t) x) in
@@ -4884,7 +4888,8 @@ Module Compilers.
   End partial.
 
   Section partial_reduce.
-    Context {var : type -> Type}.
+    Context (inline_var_nodes : bool)
+            {var : type -> Type}.
 
     Definition partial_reduce'_step
                (partial_reduce' : forall {t} (e : @expr (partial.value var) t),
@@ -4894,7 +4899,7 @@ Module Compilers.
       := match e in expr.expr t return partial.value var t with
          | Var t v => v
          | TT => inr tt
-         | AppIdent s d idc args => partial.ident.interp idc (@partial_reduce' _ args)
+         | AppIdent s d idc args => partial.ident.interp inline_var_nodes idc (@partial_reduce' _ args)
          | Pair A B a b => inr (@partial_reduce' A a, @partial_reduce' B b)
          | App s d f x => @partial_reduce' _ f (@partial_reduce' _ x)
          | Abs s d f => fun x => @partial_reduce' d (f x)
@@ -4918,8 +4923,8 @@ Module Compilers.
 
   End partial_reduce.
 
-  Definition PartialReduce {t} (e : Expr t) : Expr t
-    := fun var => @partial_reduce var t (e _).
+  Definition PartialReduce (inline_var_nodes : bool) {t} (e : Expr t) : Expr t
+    := fun var => @partial_reduce inline_var_nodes var t (e _).
 
   Module RelaxZRange.
     Module ident.
@@ -4972,7 +4977,7 @@ Module Compilers.
   Definition PartialReduceWithBounds1
              {s d} (e : Expr (s -> d)) (b : ZRange.type.interp s)
     : Expr (s -> d)
-    := fun var => @partial_reduce_with_bounds1 var s d (e _) b.
+    := fun var => @partial_reduce_with_bounds1 true var s d (e _) b.
 
   Definition CheckPartialReduceWithBounds1
              (relax_zrange : zrange -> option zrange)
@@ -5009,7 +5014,7 @@ Module Compilers.
              {t} (e : Expr t)
              (b_out : ZRange.type.interp t)
     : Expr t + ZRange.type.option.interp t
-    := dlet_nd E := PartialReduce e in
+    := dlet_nd E := PartialReduce true e in
              CheckPartialReduceWithBounds0 relax_zrange E b_out.
 
   Axiom admit_pf : False.
@@ -5048,7 +5053,7 @@ Module Compilers.
                                    -> is_tighter_than_bool z r' = true)
           {t} (e : Expr t)
           (b_out : ZRange.type.interp t)
-          E (HE : PartialReduce e = E)
+          E (HE : PartialReduce true e = E)
           rv (Hrv : CheckPartialReduceWithBounds0 relax_zrange E b_out = inl rv)
     : Interp rv = Interp e
       /\ ZRange.type.is_bounded_by b_out (Interp rv) = true.
@@ -5278,7 +5283,7 @@ Proof.
   let v := Reify ((fun x => 2^x) 255)%Z in
   pose v as E.
   vm_compute in E.
-  pose (PartialReduce (canonicalize_list_recursion E)) as E'.
+  pose (PartialReduce false (canonicalize_list_recursion E)) as E'.
   vm_compute in E'.
   lazymatch (eval cbv delta [E'] in E') with
   | (fun var => AppIdent (ident.primitive ?v) TT) => idtac
@@ -5296,7 +5301,7 @@ Module test2.
                          (fun v => v)) in
     pose v as E.
     vm_compute in E.
-    pose (PartialReduce (canonicalize_list_recursion E)) as E'.
+    pose (PartialReduce false (canonicalize_list_recursion E)) as E'.
     vm_compute in E'.
     lazymatch (eval cbv delta [E'] in E') with
     | (fun var : type -> Type =>
@@ -5329,7 +5334,7 @@ Module test3.
                         (z * z)) in
     pose v as E.
     vm_compute in E.
-    pose (PartialReduce (CPS.CallFunWithIdContinuation (CPS.Translate (canonicalize_list_recursion E)))) as E'.
+    pose (PartialReduce false (CPS.CallFunWithIdContinuation (CPS.Translate (canonicalize_list_recursion E)))) as E'.
     vm_compute in E'.
     lazymatch (eval cbv delta [E'] in E') with
     | (fun var : type -> Type =>
@@ -5366,7 +5371,7 @@ Module test4.
                         (xz :: xz :: nil)) in
     pose v as E.
     vm_compute in E.
-    pose (PartialReduce (CPS.CallFunWithIdContinuation (CPS.Translate (canonicalize_list_recursion E)))) as E'.
+    pose (PartialReduce false (CPS.CallFunWithIdContinuation (CPS.Translate (canonicalize_list_recursion E)))) as E'.
     lazy in E'.
     clear E.
     pose (PartialReduceWithBounds1 E' ([r[0~>10]%zrange],[r[0~>10]%zrange])) as E''.
@@ -5393,7 +5398,7 @@ Module test5.
                         x) in
     pose v as E.
     vm_compute in E.
-    pose (ReassociateSmallConstants.Reassociate (2^8) (PartialReduce (CPS.CallFunWithIdContinuation (CPS.Translate (canonicalize_list_recursion E))))) as E'.
+    pose (ReassociateSmallConstants.Reassociate (2^8) (PartialReduce false (CPS.CallFunWithIdContinuation (CPS.Translate (canonicalize_list_recursion E))))) as E'.
     lazy in E'.
     clear E.
     lazymatch (eval cbv delta [E'] in E') with
@@ -5420,7 +5425,7 @@ Module test6.
     pose (CPS.CallFunWithIdContinuation (CPS.Translate (canonicalize_list_recursion E))) as E'.
     lazy in E'.
     clear E.
-    pose (PartialReduce E') as E''.
+    pose (PartialReduce false E') as E''.
     lazy in E''.
     lazymatch eval cbv delta [E''] in E'' with
     | fun var : type -> Type => (λ x : var (type.type_primitive type.Z), Var x)%expr
@@ -5443,7 +5448,7 @@ Ltac cache_reify _ :=
   let e := match RHS with context[expr.Interp _ ?e] => e end in
   let E := fresh "E" in
   set (E := e);
-  let E' := constr:(PartialReduce (CPS.CallFunWithIdContinuation (CPS.Translate (canonicalize_list_recursion E)))) in
+  let E' := constr:(PartialReduce false (CPS.CallFunWithIdContinuation (CPS.Translate (canonicalize_list_recursion E)))) in
   let LHS := match goal with |- ?LHS = _ => LHS end in
   lazymatch LHS with
   | context LHS[@expr.Interp ?ident ?interp_ident ?t ?e]
@@ -5613,7 +5618,9 @@ Module Pipeline.
              {t}
              (E : for_reification.Expr t)
   : ErrorT (Expr t)
-    := let E := option_map PartialReduce (CPS.CallFunWithIdContinuation_opt (CPS.Translate (canonicalize_list_recursion E))) in
+    := let E := option_map
+                  (PartialReduce false)
+                  (CPS.CallFunWithIdContinuation_opt (CPS.Translate (canonicalize_list_recursion E))) in
        match E with
        | Some E => Success E
        | None => Error (Type_too_complicated_for_cps t)
@@ -5631,7 +5638,7 @@ Module Pipeline.
              (E : Expr (s -> d))
              arg_bounds
   : Expr (s -> d)
-    := let E := PartialReduce E in
+    := let E := PartialReduce true E in
        (* Note that DCE evaluates the expr with two different [var]
           arguments, and so will likely result in a pipeline that is
           2x slower *)
@@ -5770,13 +5777,13 @@ Module Pipeline.
              {t}
              (e : Expr t)
   : Expr t
-    := let E := PartialReduce e in
+    := let E := PartialReduce true e in
        (* Note that DCE evaluates the expr with two different [var]
           arguments, and so will likely result in a pipeline that is
           2x slower *)
        let E := if with_dead_code_elimination then DeadCodeElimination.EliminateDead E else E in
        let E := ReassociateSmallConstants.Reassociate (2^8) E in
-       let E := PartialReduce E in
+       let E := PartialReduce true E in
        E.
 
   Definition CheckBoundsPipelineConst
@@ -6637,23 +6644,68 @@ Module X25519_64.
 
   Import PrintingNotations.
   Print base_51_carry_mul.
-(* base_51_carry_mul = fun var : type -> Type => (λ v : var (type.list (type.type_primitive type.Z) * type.list (type.type_primitive type.Z))%ctype,
-expr_let v0 := (uint64)(v₁ [[0]] *₁₂₈ v₂ [[0]] +₁₂₈ (v₁ [[1]] *₁₂₈ (19 * (uint64)(v₂[[4]])) +₁₂₈ (v₁ [[2]] *₁₂₈ (19 * (uint64)(v₂[[3]])) +₁₂₈ (v₁ [[3]] *₁₂₈ (19 * (uint64)(v₂[[2]])) +₁₂₈ v₁ [[4]] *₁₂₈ (19 * (uint64)(v₂[[1]]))))) >> 51) in
-expr_let v1 := ((uint64)(v₁ [[0]] *₁₂₈ v₂ [[0]] +₁₂₈ (v₁ [[1]] *₁₂₈ (19 * (uint64)(v₂[[4]])) +₁₂₈ (v₁ [[2]] *₁₂₈ (19 * (uint64)(v₂[[3]])) +₁₂₈ (v₁ [[3]] *₁₂₈ (19 * (uint64)(v₂[[2]])) +₁₂₈ v₁ [[4]] *₁₂₈ (19 * (uint64)(v₂[[1]])))))) & 2251799813685247) in
-expr_let v2 := (uint64)((uint64)(v0) +₁₂₈ (v₁ [[0]] *₁₂₈ v₂ [[1]] +₁₂₈ (v₁ [[1]] *₁₂₈ v₂ [[0]] +₁₂₈ (v₁ [[2]] *₁₂₈ (19 * (uint64)(v₂[[4]])) +₁₂₈ (v₁ [[3]] *₁₂₈ (19 * (uint64)(v₂[[3]])) +₁₂₈ v₁ [[4]] *₁₂₈ (19 * (uint64)(v₂[[2]])))))) >> 51) in
-expr_let v3 := ((uint64)((uint64)(v0) +₁₂₈ (v₁ [[0]] *₁₂₈ v₂ [[1]] +₁₂₈ (v₁ [[1]] *₁₂₈ v₂ [[0]] +₁₂₈ (v₁ [[2]] *₁₂₈ (19 * (uint64)(v₂[[4]])) +₁₂₈ (v₁ [[3]] *₁₂₈ (19 * (uint64)(v₂[[3]])) +₁₂₈ v₁ [[4]] *₁₂₈ (19 * (uint64)(v₂[[2]]))))))) & 2251799813685247) in
-expr_let v4 := (uint64)((uint64)(v2) +₁₂₈ (v₁ [[0]] *₁₂₈ v₂ [[2]] +₁₂₈ (v₁ [[1]] *₁₂₈ v₂ [[1]] +₁₂₈ (v₁ [[2]] *₁₂₈ v₂ [[0]] +₁₂₈ (v₁ [[3]] *₁₂₈ (19 * (uint64)(v₂[[4]])) +₁₂₈ v₁ [[4]] *₁₂₈ (19 * (uint64)(v₂[[3]])))))) >> 51) in
-expr_let v5 := ((uint64)((uint64)(v2) +₁₂₈ (v₁ [[0]] *₁₂₈ v₂ [[2]] +₁₂₈ (v₁ [[1]] *₁₂₈ v₂ [[1]] +₁₂₈ (v₁ [[2]] *₁₂₈ v₂ [[0]] +₁₂₈ (v₁ [[3]] *₁₂₈ (19 * (uint64)(v₂[[4]])) +₁₂₈ v₁ [[4]] *₁₂₈ (19 * (uint64)(v₂[[3]]))))))) & 2251799813685247) in
-expr_let v6 := (uint64)((uint64)(v4) +₁₂₈ (v₁ [[0]] *₁₂₈ v₂ [[3]] +₁₂₈ (v₁ [[1]] *₁₂₈ v₂ [[2]] +₁₂₈ (v₁ [[2]] *₁₂₈ v₂ [[1]] +₁₂₈ (v₁ [[3]] *₁₂₈ v₂ [[0]] +₁₂₈ v₁ [[4]] *₁₂₈ (19 * (uint64)(v₂[[4]])))))) >> 51) in
-expr_let v7 := ((uint64)((uint64)(v4) +₁₂₈ (v₁ [[0]] *₁₂₈ v₂ [[3]] +₁₂₈ (v₁ [[1]] *₁₂₈ v₂ [[2]] +₁₂₈ (v₁ [[2]] *₁₂₈ v₂ [[1]] +₁₂₈ (v₁ [[3]] *₁₂₈ v₂ [[0]] +₁₂₈ v₁ [[4]] *₁₂₈ (19 * (uint64)(v₂[[4]]))))))) & 2251799813685247) in
-expr_let v8 := (uint64)((uint64)(v6) +₁₂₈ (v₁ [[0]] *₁₂₈ v₂ [[4]] +₁₂₈ (v₁ [[1]] *₁₂₈ v₂ [[3]] +₁₂₈ (v₁ [[2]] *₁₂₈ v₂ [[2]] +₁₂₈ (v₁ [[3]] *₁₂₈ v₂ [[1]] +₁₂₈ v₁ [[4]] *₁₂₈ v₂ [[0]])))) >> 51) in
-expr_let v9 := ((uint64)((uint64)(v6) +₁₂₈ (v₁ [[0]] *₁₂₈ v₂ [[4]] +₁₂₈ (v₁ [[1]] *₁₂₈ v₂ [[3]] +₁₂₈ (v₁ [[2]] *₁₂₈ v₂ [[2]] +₁₂₈ (v₁ [[3]] *₁₂₈ v₂ [[1]] +₁₂₈ v₁ [[4]] *₁₂₈ v₂ [[0]]))))) & 2251799813685247) in
-expr_let v10 := (uint64)((uint64)(v1) +₆₄ 19 *₆₄ (uint64)(v8) >> 51) in
-expr_let v11 := ((uint64)((uint64)(v1) +₆₄ 19 *₆₄ (uint64)(v8)) & 2251799813685247) in
-expr_let v12 := (uint64)((uint64)(v10) +₆₄ (uint64)(v3) >> 51) in
-expr_let v13 := ((uint64)((uint64)(v10) +₆₄ (uint64)(v3)) & 2251799813685247) in
-(uint64)(v11) :: (uint64)(v13) :: (uint64)(v12) +₆₄ (uint64)(v5) :: (uint64)(v7) :: (uint64)(v9) :: [])%expr
-     : Expr (type.list (type.type_primitive type.Z) * type.list (type.type_primitive type.Z) -> type.list (type.type_primitive type.Z))
+(*base_51_carry_mul =
+fun var : type -> Type =>
+(λ v : var
+         (type.list (type.type_primitive type.Z) *
+          type.list (type.type_primitive type.Z))%ctype,
+ expr_let v0 := v₁ [[4]] *₁₂₈ (19 * (uint64)(v₂[[4]])) in
+ expr_let v1 := v₁ [[4]] *₁₂₈ (19 * (uint64)(v₂[[3]])) in
+ expr_let v2 := v₁ [[4]] *₁₂₈ (19 * (uint64)(v₂[[2]])) in
+ expr_let v3 := v₁ [[4]] *₁₂₈ (19 * (uint64)(v₂[[1]])) in
+ expr_let v4 := v₁ [[3]] *₁₂₈ (19 * (uint64)(v₂[[4]])) in
+ expr_let v5 := v₁ [[3]] *₁₂₈ (19 * (uint64)(v₂[[3]])) in
+ expr_let v6 := v₁ [[3]] *₁₂₈ (19 * (uint64)(v₂[[2]])) in
+ expr_let v7 := v₁ [[2]] *₁₂₈ (19 * (uint64)(v₂[[4]])) in
+ expr_let v8 := v₁ [[2]] *₁₂₈ (19 * (uint64)(v₂[[3]])) in
+ expr_let v9 := v₁ [[1]] *₁₂₈ (19 * (uint64)(v₂[[4]])) in
+ expr_let v10 := v₁ [[4]] *₁₂₈ v₂ [[0]] in
+ expr_let v11 := v₁ [[3]] *₁₂₈ v₂ [[1]] in
+ expr_let v12 := v₁ [[3]] *₁₂₈ v₂ [[0]] in
+ expr_let v13 := v₁ [[2]] *₁₂₈ v₂ [[2]] in
+ expr_let v14 := v₁ [[2]] *₁₂₈ v₂ [[1]] in
+ expr_let v15 := v₁ [[2]] *₁₂₈ v₂ [[0]] in
+ expr_let v16 := v₁ [[1]] *₁₂₈ v₂ [[3]] in
+ expr_let v17 := v₁ [[1]] *₁₂₈ v₂ [[2]] in
+ expr_let v18 := v₁ [[1]] *₁₂₈ v₂ [[1]] in
+ expr_let v19 := v₁ [[1]] *₁₂₈ v₂ [[0]] in
+ expr_let v20 := v₁ [[0]] *₁₂₈ v₂ [[4]] in
+ expr_let v21 := v₁ [[0]] *₁₂₈ v₂ [[3]] in
+ expr_let v22 := v₁ [[0]] *₁₂₈ v₂ [[2]] in
+ expr_let v23 := v₁ [[0]] *₁₂₈ v₂ [[1]] in
+ expr_let v24 := v₁ [[0]] *₁₂₈ v₂ [[0]] in
+ expr_let v25 := v24 +₁₂₈ (v9 +₁₂₈ (v8 +₁₂₈ (v6 +₁₂₈ v3))) in
+ expr_let v26 := (uint64)(v25 >> 51) in
+ expr_let v27 := ((uint64)(v25) & 2251799813685247) in
+ expr_let v28 := v20 +₁₂₈ (v16 +₁₂₈ (v13 +₁₂₈ (v11 +₁₂₈ v10))) in
+ expr_let v29 := v21 +₁₂₈ (v17 +₁₂₈ (v14 +₁₂₈ (v12 +₁₂₈ v0))) in
+ expr_let v30 := v22 +₁₂₈ (v18 +₁₂₈ (v15 +₁₂₈ (v4 +₁₂₈ v1))) in
+ expr_let v31 := v23 +₁₂₈ (v19 +₁₂₈ (v7 +₁₂₈ (v5 +₁₂₈ v2))) in
+ expr_let v32 := v26 +₁₂₈ v31 in
+ expr_let v33 := (uint64)(v32 >> 51) in
+ expr_let v34 := ((uint64)(v32) & 2251799813685247) in
+ expr_let v35 := v33 +₁₂₈ v30 in
+ expr_let v36 := (uint64)(v35 >> 51) in
+ expr_let v37 := ((uint64)(v35) & 2251799813685247) in
+ expr_let v38 := v36 +₁₂₈ v29 in
+ expr_let v39 := (uint64)(v38 >> 51) in
+ expr_let v40 := ((uint64)(v38) & 2251799813685247) in
+ expr_let v41 := v39 +₁₂₈ v28 in
+ expr_let v42 := (uint64)(v41 >> 51) in
+ expr_let v43 := ((uint64)(v41) & 2251799813685247) in
+ expr_let v44 := 19 *₆₄ v42 in
+ expr_let v45 := v27 +₆₄ v44 in
+ expr_let v46 := (uint64)(v45 >> 51) in
+ expr_let v47 := ((uint64)(v45) & 2251799813685247) in
+ expr_let v48 := v46 +₆₄ v34 in
+ expr_let v49 := (uint64)(v48 >> 51) in
+ expr_let v50 := ((uint64)(v48) & 2251799813685247) in
+ expr_let v51 := v49 +₆₄ v37 in
+ v47 :: v50 :: v51 :: v40 :: v43 :: [])%expr
+     : Expr
+         (type.list (type.type_primitive type.Z) *
+          type.list (type.type_primitive type.Z) ->
+          type.list (type.type_primitive type.Z))
 *)
 End X25519_64.
 
